PAC/PAC_Checker_Init.thy
@@ -317,4 +317,362 @@ sepref_definition normalize_poly_impl
 declare normalize_poly_impl.refine[sepref_fr_rules]
 
 
+definition full_quicksort_vars where
+  \<open>full_quicksort_vars = full_quicksort_ref (\<lambda>x y. x = y \<or> (x, y) \<in> var_order_rel) id\<close>
+
+
+definition quicksort_vars:: \<open>nat \<Rightarrow> nat \<Rightarrow> string list \<Rightarrow> (string list) nres\<close> where
+  \<open>quicksort_vars x y  z = quicksort_ref (\<le>) id (x, y, z)\<close>
+
+term partition_between_ref
+
+definition partition_between_vars :: \<open>nat \<Rightarrow> nat \<Rightarrow> string list \<Rightarrow> (string list \<times> nat) nres\<close> where
+  \<open>partition_between_vars = partition_between_ref (\<le>) id\<close>
+
+definition partition_main_vars :: \<open>nat \<Rightarrow> nat \<Rightarrow> string list \<Rightarrow> (string list \<times> nat) nres\<close> where
+  \<open>partition_main_vars = partition_main (\<le>) id\<close>
+
+lemma total_on_lexord_less_than_char_linear2:
+  \<open>xs \<noteq> ys \<Longrightarrow> (xs, ys) \<notin> lexord (less_than_char) \<longleftrightarrow>
+       (ys, xs) \<in> lexord less_than_char\<close>
+   using lexord_linear[of \<open>less_than_char\<close> xs ys]
+   using lexord_linear[of \<open>less_than_char\<close>] less_than_char_linear
+   apply (auto simp: Relation.total_on_def)
+   using lexord_irrefl[OF irrefl_less_than_char]
+     antisym_lexord[OF antisym_less_than_char irrefl_less_than_char]
+   apply (auto simp: antisym_def)
+   done
+
+lemma full_quicksort_sort_vars_spec:
+  \<open>(full_quicksort_vars, sort_coeff) \<in> \<langle>Id\<rangle>list_rel \<rightarrow>\<^sub>f \<langle>\<langle>Id\<rangle>list_rel\<rangle>nres_rel\<close>
+proof -
+  have xs: \<open>(xs, xs) \<in> \<langle>Id\<rangle>list_rel\<close> and \<open>\<Down>(\<langle>Id\<rangle>list_rel) x = x\<close> for x xs
+    by auto
+  show ?thesis
+    apply (intro frefI nres_relI)
+    unfolding full_quicksort_vars_def
+    apply (rule full_quicksort_ref_full_quicksort[THEN fref_to_Down_curry, THEN order_trans])
+    subgoal
+      apply (auto simp: rel2p_def var_order_rel_def p2rel_def Relation.total_on_def)
+      apply (smt less_char_def char.less_trans less_than_char_def lexord_partial_trans p2rel_def)
+      done
+    subgoal
+      using total_on_lexord_less_than_char_linear2[unfolded var_order_rel_def]
+      apply (auto simp: rel2p_def var_order_rel_def p2rel_def Relation.total_on_def less_char_def)
+      done
+    subgoal by fast
+    apply (rule xs)
+    apply (subst down_eq_id_list_rel)
+    unfolding sorted_wrt_map sort_coeff_def
+    apply (rule full_quicksort_correct_sorted[where R = \<open>(\<lambda>x y. x = y \<or> (x, y) \<in> var_order_rel)\<close> and h = \<open>id\<close>,
+       THEN order_trans])
+    subgoal
+      apply (auto simp: rel2p_def var_order_rel_def p2rel_def Relation.total_on_def)
+      apply (smt less_char_def char.less_trans less_than_char_def lexord_partial_trans p2rel_def)
+      done
+    subgoal for x y
+      using total_on_lexord_less_than_char_linear2[unfolded var_order_rel_def]
+      apply (auto simp: rel2p_def var_order_rel_def p2rel_def Relation.total_on_def
+        less_char_def)
+      done
+   subgoal
+    by (auto simp: rel2p_def p2rel_def rel2p_def[abs_def])
+   done
+qed
+
+definition var_order' where
+  [simp]: \<open>var_order' = var_order\<close>
+
+lemma var_order_rel[def_pat_rules]:
+  \<open>(\<in>)$(x,y)$var_order_rel \<equiv> var_order'$x$y\<close>
+  by (auto simp: p2rel_def rel2p_def)
+
+lemma var_order_rel_alt_def:
+  \<open>var_order_rel = p2rel char.lexordp\<close>
+  apply (auto simp: p2rel_def char.lexordp_conv_lexord var_order_rel_def)
+  using char.lexordp_conv_lexord apply auto
+  done
+
+lemma var_order_rel_var_order:
+  \<open>(x, y) \<in> var_order_rel \<longleftrightarrow> var_order x y\<close>
+  by (auto simp: rel2p_def)
+
+lemma var_order_string_le[sepref_import_param]:
+  \<open>((<), var_order') \<in> string_rel \<rightarrow> string_rel \<rightarrow> bool_rel\<close>
+  apply (auto intro!: frefI simp: string_rel_def String.less_literal_def
+     rel2p_def linorder.lexordp_conv_lexord[OF char.linorder_axioms,
+      unfolded less_eq_char_def] var_order_rel_def
+      p2rel_def
+      simp flip: PAC_Polynoms_Term.less_char_def)
+  using char.lexordp_conv_lexord apply auto
+  done
+
+lemma [sepref_import_param]:
+  \<open>( (\<le>), (\<le>)) \<in> monom_rel \<rightarrow> monom_rel \<rightarrow>bool_rel\<close>
+  apply (intro fun_relI)
+  using list_rel_list_rel_order_iff by fastforce
+
+lemma [sepref_import_param]:
+  \<open>( (\<le>), (\<le>)) \<in> string_rel \<rightarrow> string_rel \<rightarrow>bool_rel\<close>
+  unfolding string_rel_def less_eq_literal.rep_eq less_than_char_def
+    less_eq_list_def PAC_Polynoms_Term.less_char_def[symmetric]
+  by (intro fun_relI)
+   (auto simp: string_rel_def less_eq_literal.rep_eq less_than_char_def
+    less_eq_list_def char.lexordp_eq_conv_lexord lexordp_eq_refl
+    lexord_code lexordp_eq_conv_lexord
+    simp flip: less_char_def[abs_def])
+
+
+sepref_definition partition_main_vars_impl
+  is \<open>uncurry2 partition_main_vars\<close>
+  :: \<open>nat_assn\<^sup>k *\<^sub>a nat_assn\<^sup>k *\<^sub>a (monom_assn)\<^sup>k \<rightarrow>\<^sub>a prod_assn (monom_assn) nat_assn\<close>
+  unfolding partition_main_vars_def partition_main_def
+    var_order_rel_var_order
+    var_order'_def[symmetric]
+    term_order_rel'_alt_def
+    le_term_order_rel'
+    id_apply
+    by sepref
+
+declare partition_main_vars_impl.refine[sepref_fr_rules]
+
+sepref_definition partition_between_vars_impl
+  is \<open>uncurry2 partition_between_vars\<close>
+  :: \<open>nat_assn\<^sup>k *\<^sub>a nat_assn\<^sup>k *\<^sub>a monom_assn\<^sup>k \<rightarrow>\<^sub>a prod_assn monom_assn nat_assn \<close>
+  unfolding partition_between_vars_def partition_between_ref_def
+    partition_main_vars_def[symmetric]
+  unfolding choose_pivot3_def
+    term_order_rel'_def[symmetric]
+    term_order_rel'_alt_def choose_pivot_def
+    le_term_order_rel' id_apply
+  by sepref
+
+declare partition_between_vars_impl.refine[sepref_fr_rules]
+
+sepref_definition quicksort_vars_impl
+  is \<open>uncurry2 quicksort_vars\<close>
+  :: \<open>nat_assn\<^sup>k *\<^sub>a nat_assn\<^sup>k *\<^sub>a monom_assn\<^sup>k \<rightarrow>\<^sub>a monom_assn\<close>
+  unfolding partition_main_vars_def quicksort_ref_def quicksort_vars_def
+    partition_between_vars_def[symmetric]
+  by sepref
+
+lemmas [sepref_fr_rules] = quicksort_vars_impl.refine
+
+sepref_register quicksort_vars
+
+
+lemma le_var_order_rel:
+  \<open>(\<le>) = (\<lambda>x y. x = y \<or> (x, y) \<in> var_order_rel)\<close>
+  by (intro ext)
+   (auto simp add: less_list_def less_eq_list_def rel2p_def
+      p2rel_def lexordp_conv_lexord p2rel_def var_order_rel_def
+    lexordp_eq_conv_lexord lexordp_def)
+
+sepref_definition full_quicksort_vars_impl
+  is \<open>full_quicksort_vars\<close>
+  :: \<open>monom_assn\<^sup>k \<rightarrow>\<^sub>a monom_assn\<close>
+  unfolding full_quicksort_vars_def full_quicksort_ref_def
+    quicksort_vars_def[symmetric]
+    le_var_order_rel[symmetric]
+    term_order_rel'_def[symmetric]
+    List.null_def
+  by sepref
+
+
+lemmas sort_vars_spec_hnr[sepref_fr_rules] =
+  full_quicksort_vars_impl.refine[FCOMP full_quicksort_sort_vars_spec]
+
+
+sepref_definition sort_all_coeffs_impl
+  is \<open>sort_all_coeffs\<close>
+  :: \<open>poly_assn\<^sup>k \<rightarrow>\<^sub>a poly_assn\<close>
+  unfolding sort_all_coeffs_def
+    HOL_list.fold_custom_empty
+  by sepref
+
+declare sort_all_coeffs_impl.refine[sepref_fr_rules]
+
+lemma merge_coeffs0_alt_def:
+  \<open>(RETURN o merge_coeffs0) p =
+   REC\<^sub>T(\<lambda>f p.
+     (case p of
+       [] \<Rightarrow> RETURN []
+     | [p] => if snd p = 0 then RETURN [] else RETURN [p]
+     | ((xs, n) # (ys, m) # p) \<Rightarrow>
+      (if xs = ys
+       then if n + m \<noteq> 0 then f ((xs, n + m) # p) else f p
+       else if n = 0 then
+          do {p \<leftarrow> f ((ys, m) # p);
+            RETURN p}
+       else do {p \<leftarrow> f ((ys, m) # p);
+            RETURN ((xs, n) # p)})))
+    p\<close>
+  apply (induction p rule: merge_coeffs0.induct)
+  subgoal
+    apply (subst RECT_unfold)
+    apply refine_mono
+    apply auto
+    done
+  subgoal
+    apply (subst RECT_unfold)
+    apply refine_mono
+    apply (cases p)
+    apply auto
+    done
+  subgoal for x p y q
+    apply (subst RECT_unfold)
+    apply refine_mono
+    apply (auto simp: let_to_bind_conv)
+    apply (metis let_to_bind_conv)+
+    done
+  done
+
+
+sepref_definition merge_coeffs0_impl
+  is \<open>RETURN o merge_coeffs0\<close>
+  :: \<open>poly_assn\<^sup>k \<rightarrow>\<^sub>a poly_assn\<close>
+  supply [[goals_limit=1]]
+  unfolding merge_coeffs0_alt_def
+    HOL_list.fold_custom_empty
+  apply sepref_dbg_preproc
+  apply sepref_dbg_cons_init
+  apply sepref_dbg_id
+  apply sepref_dbg_monadify
+  apply sepref_dbg_opt_init
+  apply sepref_dbg_trans_step
+  apply sepref_dbg_trans_step
+  apply sepref_dbg_trans_step
+  apply sepref_dbg_trans_step
+  apply sepref_dbg_trans_step
+  apply sepref_dbg_trans_step
+  apply sepref_dbg_trans_step
+  apply sepref_dbg_trans_step
+  apply sepref_dbg_trans_step
+  apply sepref_dbg_trans_step
+  apply sepref_dbg_trans_step
+  apply sepref_dbg_trans_step
+  apply sepref_dbg_trans_step
+  apply sepref_dbg_trans_step
+  apply sepref_dbg_trans_step
+  apply sepref_dbg_trans_step
+  apply sepref_dbg_trans_step
+  apply sepref_dbg_trans_step
+  apply sepref_dbg_trans_step
+  apply sepref_dbg_trans_step
+  apply sepref_dbg_trans_step
+  apply sepref_dbg_trans_step
+  apply sepref_dbg_trans_step
+  apply sepref_dbg_trans_step
+  apply sepref_dbg_trans_step
+  apply sepref_dbg_trans_step
+  apply sepref_dbg_trans_step
+  apply sepref_dbg_trans_step
+  apply sepref_dbg_trans_step
+  apply sepref_dbg_trans_step
+  apply sepref_dbg_trans_step
+  apply sepref_dbg_trans_step
+  apply sepref_dbg_trans_step
+  apply sepref_dbg_trans_step
+  apply sepref_dbg_trans_step
+  apply sepref_dbg_trans_step
+  apply sepref_dbg_trans_step
+  apply sepref_dbg_trans_step
+  apply sepref_dbg_trans_step
+  apply sepref_dbg_trans_step
+  apply sepref_dbg_trans_step
+  apply sepref_dbg_trans_step
+  apply sepref_dbg_trans_step
+  apply sepref_dbg_trans_step
+  apply sepref_dbg_trans_step
+  apply sepref_dbg_trans_step
+  apply sepref_dbg_trans_step
+  apply sepref_dbg_trans_step
+  apply sepref_dbg_trans_step
+  apply sepref_dbg_trans_step
+  apply sepref_dbg_trans_step
+  apply sepref_dbg_trans_step
+  apply sepref_dbg_trans_step
+  apply sepref_dbg_trans_step
+  apply sepref_dbg_trans_step
+  apply sepref_dbg_trans_step
+  apply sepref_dbg_trans_step
+  apply sepref_dbg_trans_step
+  apply sepref_dbg_trans_step
+  apply sepref_dbg_trans_step
+  apply sepref_dbg_trans_step
+  apply sepref_dbg_trans_step
+  apply sepref_dbg_trans_step
+  apply sepref_dbg_trans_step
+  apply sepref_dbg_trans_step
+  apply sepref_dbg_trans_step
+  apply sepref_dbg_trans_step
+  apply sepref_dbg_trans_step
+  apply sepref_dbg_trans_step
+  apply sepref_dbg_trans_step
+  apply sepref_dbg_trans_step
+  apply sepref_dbg_trans_step
+  apply sepref_dbg_trans_step
+  apply sepref_dbg_trans_step
+  apply sepref_dbg_trans_step
+  apply sepref_dbg_trans_step
+  apply sepref_dbg_trans_step
+  apply sepref_dbg_trans_step
+  apply sepref_dbg_trans_step
+  apply sepref_dbg_trans_step
+  apply sepref_dbg_trans_step
+  apply sepref_dbg_trans_step
+  apply sepref_dbg_trans_step
+  apply sepref_dbg_trans_step
+  apply sepref_dbg_trans_step
+  apply sepref_dbg_trans_step
+  apply sepref_dbg_trans_step
+  apply sepref_dbg_trans_step
+  apply sepref_dbg_trans_step
+  apply sepref_dbg_trans_step
+  apply sepref_dbg_trans_step
+  apply sepref_dbg_trans_step
+  apply sepref_dbg_trans_step
+  apply sepref_dbg_trans_step
+  apply sepref_dbg_trans_step
+  apply sepref_dbg_trans_step
+  apply sepref_dbg_trans_step
+  apply sepref_dbg_trans_step
+  apply sepref_dbg_trans_step
+  apply sepref_dbg_trans_step
+  apply sepref_dbg_trans_step
+  apply sepref_dbg_trans_step
+  apply sepref_dbg_trans_step
+  apply sepref_dbg_trans_step
+  apply sepref_dbg_trans_step
+  apply sepref_dbg_trans_step
+  apply sepref_dbg_trans_step
+  apply sepref_dbg_trans_step
+  apply sepref_dbg_trans_step
+  apply (rule WTF_RF)
+  apply sepref_dbg_trans_step
+  apply sepref_dbg_trans_step
+  apply sepref_dbg_trans_step
+  apply (rule WTF_RF)
+  apply sepref_dbg_trans_step
+  apply sepref_dbg_trans_step
+  apply sepref_dbg_trans_step
+  apply sepref_dbg_trans_step
+  apply sepref_dbg_opt
+  apply sepref_dbg_cons_solve
+  apply sepref_dbg_cons_solve
+  apply sepref_dbg_constraints
+  done
+
+
+declare merge_coeffs0_impl.refine[sepref_fr_rules]
+
+sepref_definition fully_normalize_poly_impl
+  is \<open>full_normalize_poly\<close>
+  :: \<open>poly_assn\<^sup>k \<rightarrow>\<^sub>a poly_assn\<close>
+  supply [[goals_limit=1]]
+  unfolding full_normalize_poly_def
+  by sepref
+
+declare fully_normalize_poly_impl.refine[sepref_fr_rules]
+
 end
